simplify expr metrics WIP

bedrock2/src/Semantics.v
@@ -126,50 +126,32 @@ Section semantics.
 
   Section WithMemAndLocals.
     Context (m : mem) (l : locals).
-    Fixpoint eval_expr (e : expr) (mc : metrics) : option (word * metrics) :=
-      match e with
-      | expr.literal v => Some (word.of_Z v, addMetricInstructions 8
-                                             (addMetricLoads 8 mc))
-      | expr.var x => match map.get l x with
-                      | Some v => Some (v, addMetricInstructions 1
-                                           (addMetricLoads 2 mc))
-                      | None => None
-                      end
-      | expr.load aSize a =>
-          'Some (a', mc') <- eval_expr a mc | None;
-          'Some v <- load aSize m a' | None;
-          Some (v, addMetricInstructions 1
-                   (addMetricLoads 2 mc'))
-      | expr.op op e1 e2 =>
-          'Some (v1, mc') <- eval_expr e1 mc | None;
-          'Some (v2, mc'') <- eval_expr e2 mc' | None;
-          Some (interp_binop op v1 v2, addMetricInstructions 2
-                                       (addMetricLoads 2 mc''))
-      end.
-
-    Fixpoint eval_expr_old (e : expr) : option word :=
+    Fixpoint eval_expr (e : expr) : option word :=
       match e with
       | expr.literal v => Some (word.of_Z v)
       | expr.var x => map.get l x
       | expr.load aSize a =>
-          'Some a' <- eval_expr_old a | None;
+          'Some a' <- eval_expr a | None;
           load aSize m a'
       | expr.op op e1 e2 =>
-          'Some v1 <- eval_expr_old e1 | None;
-          'Some v2 <- eval_expr_old e2 | None;
+          'Some v1 <- eval_expr e1 | None;
+          'Some v2 <- eval_expr e2 | None;
           Some (interp_binop op v1 v2)
       end.
-
-    Fixpoint evaluate_call_args_log (arges : list expr) (mc : metrics) :=
-      match arges with
-      | e :: tl =>
-        'Some (v, mc') <- eval_expr e mc | None;
-        'Some (args, mc'') <- evaluate_call_args_log tl mc' | None;
-        Some (v :: args, mc'')
-      | _ => Some (nil, mc)
-      end.
-
   End WithMemAndLocals.
+
+  Fixpoint measure_expr (e : expr) (mc : metrics) : metrics :=
+    match e with
+    | expr.literal v => addMetricInstructions 8 (addMetricLoads 8 mc)
+    | expr.var x => addMetricInstructions 1 (addMetricLoads 2 mc)
+    | expr.load aSize a => addMetricInstructions 1 (addMetricLoads 2 (measure_expr a mc))
+    | expr.op op e1 e2 => addMetricInstructions 2 (addMetricLoads 2 (measure_expr e2 (measure_expr e1 mc)))
+    end.
+  Fixpoint measure_args (arges : list expr) (mc : metrics) :=
+    match arges with
+    | e :: tl => measure_args tl (measure_expr e mc)
+    | _ => mc
+    end.
 End semantics.
 
 Module exec. Section WithEnv.
@@ -187,9 +169,9 @@ Module exec. Section WithEnv.
     : exec cmd.skip t m l mc post
   | set x e
     t m l mc post
-    v mc' (_ : eval_expr m l e mc = Some (v, mc'))
+    v (_ : eval_expr m l e = Some v)
     (_ : post t m (map.put l x v) (addMetricInstructions 1
-                                  (addMetricLoads 1 mc')))
+                                  (addMetricLoads 1 (measure_expr e mc))))
     : exec (cmd.set x e) t m l mc post
   | unset x
     t m l mc post
@@ -197,27 +179,27 @@ Module exec. Section WithEnv.
     : exec (cmd.unset x) t m l mc post
   | store sz ea ev
     t m l mc post
-    a mc' (_ : eval_expr m l ea mc = Some (a, mc'))
-    v mc'' (_ : eval_expr m l ev mc' = Some (v, mc''))
+    a (_ : eval_expr m l ea = Some a)
+    v (_ : eval_expr m l ev = Some v)
     m' (_ : store sz m a v = Some m')
     (_ : post t m' l (addMetricInstructions 1
                      (addMetricLoads 1
-                     (addMetricStores 1 mc''))))
+                     (addMetricStores 1 (measure_expr ev (measure_expr ea mc))))))
     : exec (cmd.store sz ea ev) t m l mc post
   | if_true t m l mc e c1 c2 post
-    v mc' (_ : eval_expr m l e mc = Some (v, mc'))
+    v (_ : eval_expr m l e = Some v)
     (_ : word.unsigned v <> 0)
     (_ : exec c1 t m l (addMetricInstructions 2
                        (addMetricLoads 2
-                       (addMetricJumps 1 mc'))) post)
+                       (addMetricJumps 1 (measure_expr e mc)))) post)
     : exec (cmd.cond e c1 c2) t m l mc post
   | if_false e c1 c2
     t m l mc post
-    v mc' (_ : eval_expr m l e mc = Some (v, mc'))
+    v (_ : eval_expr m l e = Some v)
     (_ : word.unsigned v = 0)
     (_ : exec c2 t m l (addMetricInstructions 2
                        (addMetricLoads 2
-                       (addMetricJumps 1 mc'))) post)
+                       (addMetricJumps 1 (measure_expr e mc)))) post)
     : exec (cmd.cond e c1 c2) t m l mc post
   | seq c1 c2
     t m l mc post
@@ -226,37 +208,37 @@ Module exec. Section WithEnv.
     : exec (cmd.seq c1 c2) t m l mc post
   | while_false e c
     t m l mc post
-    v mc' (_ : eval_expr m l e mc = Some (v, mc'))
+    v (_ : eval_expr m l e = Some v)
     (_ : word.unsigned v = 0)
     (_ : post t m l (addMetricInstructions 1
                     (addMetricLoads 1
-                    (addMetricJumps 1 mc'))))
+                    (addMetricJumps 1 (measure_expr e mc)))))
     : exec (cmd.while e c) t m l mc post
   | while_true e c
       t m l mc post
-      v mc' (_ : eval_expr m l e mc = Some (v, mc'))
+      v (_ : eval_expr m l e = Some v)
       (_ : word.unsigned v <> 0)
-      mid (_ : exec c t m l mc' mid)
-      (_ : forall t' m' l' mc'', mid t' m' l' mc'' ->
+      mid (_ : exec c t m l (measure_expr e mc) mid)
+      (_ : forall t' m' l' mc', mid t' m' l' mc' ->
                                  exec (cmd.while e c) t' m' l' (addMetricInstructions 2
                                                                (addMetricLoads 2
-                                                               (addMetricJumps 1 mc''))) post)
+                                                               (addMetricJumps 1 mc'))) post)
     : exec (cmd.while e c) t m l mc post
   | call binds fname arges
       t m l mc post
       params rets fbody (_ : map.get e fname = Some (params, rets, fbody))
-      args mc' (_ : evaluate_call_args_log m l arges mc = Some (args, mc'))
+      args (_ : List.option_all (List.map (eval_expr m l) arges) = Some args)
       lf (_ : map.putmany_of_list params args map.empty = Some lf)
-      mid (_ : exec fbody t m lf mc' mid)
-      (_ : forall t' m' st1 mc'', mid t' m' st1 mc'' ->
+      mid (_ : exec fbody t m lf (measure_args arges mc) mid)
+      (_ : forall t' m' st1 mc', mid t' m' st1 mc' ->
           exists retvs, map.getmany_of_list st1 rets = Some retvs /\
           exists l', map.putmany_of_list binds retvs l = Some l' /\
-          post t' m' l' mc'')
+          post t' m' l' mc')
     : exec (cmd.call binds fname arges) t m l mc post
   | interact binds action arges
       t m l mc post
       mKeep mGive (_: map.split m mKeep mGive)
-      args mc' (_ :  evaluate_call_args_log m l arges mc = Some (args, mc'))
+      args (_ : List.option_all (List.map (eval_expr m l) arges) = Some args)
       mid (_ : ext_spec t mGive action args mid)
       (_ : forall mReceive resvals, mid mReceive resvals ->
           exists l', map.putmany_of_list binds resvals l = Some l' /\
@@ -264,7 +246,7 @@ Module exec. Section WithEnv.
                      post (cons ((mGive, action, args), (mReceive, resvals)) t) m' l'
                        (addMetricInstructions 1
                        (addMetricStores 1
-                       (addMetricLoads 2 mc'))))
+                       (addMetricLoads 2 (measure_args arges mc)))))
     : exec (cmd.interact binds action arges) t m l mc post
   .
   End WithEnv.
